boogieamp/src/boogie/declaration/Implementation.java
@@ -30,5 +30,63 @@ public class Implementation extends ProcedureOrImplementationDeclaration {
 
 	}
 	
+	/**
+	 * Returns a textual description of this object.
+	 */
+	public String toString() {
+		StringBuffer sb = new StringBuffer();
+		sb.append("Implementation").append('[');
+		sb.append(identifier);
+		sb.append(',');
+		if (typeParams == null) {
+			sb.append("null");
+		} else {
+			sb.append('[');
+			for (int i1 = 0; i1 < typeParams.length; i1++) {
+				if (i1 > 0)
+					sb.append(',');
+				sb.append(typeParams[i1]);
+			}
+			sb.append(']');
+		}
+		sb.append(',');
+		if (inParams == null) {
+			sb.append("null");
+		} else {
+			sb.append('[');
+			for (int i1 = 0; i1 < inParams.length; i1++) {
+				if (i1 > 0)
+					sb.append(',');
+				sb.append(inParams[i1]);
+			}
+			sb.append(']');
+		}
+		sb.append(',');
+		if (outParams == null) {
+			sb.append("null");
+		} else {
+			sb.append('[');
+			for (int i1 = 0; i1 < outParams.length; i1++) {
+				if (i1 > 0)
+					sb.append(',');
+				sb.append(outParams[i1]);
+			}
+			sb.append(']');
+		}
+		sb.append(',');
+		if (specification == null) {
+			sb.append("null");
+		} else {
+			sb.append('[');
+			for (int i1 = 0; i1 < specification.length; i1++) {
+				if (i1 > 0)
+					sb.append(',');
+				sb.append(specification[i1]);
+			}
+			sb.append(']');
+		}
+		sb.append(',').append(body);
+		return sb.append(']').toString();
+	}
 
 }
