boogieamp/test/divmod.bpl
@@ -1,57 +1,38 @@
-
 type ref;
 type javaType;
-const unique $null : ref;
-
 type Field $GenericType__0;
-
 type $heap_type = <$GenericType__0>[ref,Field $GenericType__0]$GenericType__0;
-
-var $heap : $heap_type;
-
-
-
-
-
-
-//$type is used to store the type of a java object on the heap.
-//E.g., String s will have $heap[s,$type]==string
+type boolArrHeap_type = [ref][int]bool;
+type refArrHeap_type = [ref][int]ref;
+type realArrHeap_type = [ref][int]int;
+type intArrHeap_type = [ref][int]int;
+const unique $null : ref;
 const unique $type : Field javaType;
-//$heap[s,$alloc] is true if s is properly allocated
-const unique $alloc : Field bool ;
-
-
+const unique $alloc : Field bool;
+const unique java.lang.Object : javaType extends  complete;
+const unique NullPointerExceptions : javaType extends  unique java.lang.Object complete;
+const unique java.io.Serializable : javaType extends  unique java.lang.Object complete;
+const unique java.lang.Throwable : javaType extends  unique java.lang.Object, unique java.io.Serializable complete;
+const unique java.lang.Exception : javaType extends  unique java.lang.Throwable complete;
+const unique java.lang.RuntimeException : javaType extends  unique java.lang.Exception complete;
+const unique java.lang.NullPointerException : javaType extends  unique java.lang.RuntimeException complete;
+var $heap : $heap_type;
+var $intArrayType : javaType;
+var $charArrayType : javaType;
 var $boolArrayType : javaType;
 var $byteArrayType : javaType;
 var $longArrayType : javaType;
-
-//an array that stores the size of java arrays.
 var $arrSizeHeap : [ref]int;
-
-//an array that stores the size of java string.
 var $stringSizeHeap : [ref]int;
-
-
-
-var $boolArrHeap : [ref][int]bool;
-var $refArrHeap : [ref][int]ref;
-var $realArrHeap : [ref][int]int;
-var $intArrHeap : [ref][int]int;
-
-
-//helper functions to cast between types.
-//this is necessary because java bytecode does not distinguish between
-//int and bool.
+var $boolArrHeap : boolArrHeap_type;
+var $refArrHeap : refArrHeap_type;
+var $realArrHeap : realArrHeap_type;
+var $intArrHeap : intArrHeap_type;
+function $arrayType(t:javaType) returns ($ret:javaType);
 function $intToReal(x:int) returns ($ret:real);
 function $intToBool(x:int) returns ($ret:bool) { (if x == 0 then false else true) }
 function $refToBool(x:ref) returns ($ret:bool) { (if x == $null then false else true) }
 function $boolToInt(x:bool) returns ($ret:int) { (if x == true then 1 else 0) }
-
-
-function $arrayType(t:javaType) returns ($ret:javaType);
-var $intArrayType : javaType;
-var $charArrayType : javaType;
-
 function $cmpBool(x:bool, y:bool) returns ($ret:int);
 function $cmpRef(x:ref, y:ref) returns ($ret:int);
 function $cmpReal(x:real, y:real) returns ($ret:int) { (if x > y then 1 else (if x < y then -1 else 0)) }
@@ -62,24 +43,86 @@ function $xorInt(x:int, y:int) returns ($ret:int);
 function $shlInt(x:int, y:int) returns ($ret:int);
 function $ushrInt(x:int, y:int) returns ($ret:int);
 function $shrInt(x:int, y:int) returns ($ret:int);
+procedure java.lang.Object$java.lang.Object$clone$43($this:ref) returns ($other:ref, $exception:ref)    modifies $heap;{
+    havoc $other;
+    assume !$heap[$other,$alloc];
+    $heap := $heap[$other,$alloc := true];
+    assume $other != $null;
+    $heap := $heap[$other,$type := $heap[$this,$type]];
+}
 
 
+procedure int$java.lang.String$compareTo$87($this:ref, $other:ref) returns ($return:int, $exception:ref);        ensures ($this == $other ==> $return == 1) && ($this != $other ==> $return == 0);
+
+procedure void$NullPointerExceptions$add$1889($this:ref) returns ($exception:ref);    
+
+procedure void$NullPointerExceptions$test$1890($this:ref) returns ($exception:ref);    
+
+procedure void$NullPointerExceptions$$la$init$ra$$1891($this:ref) returns ($exception:ref);    
+
+procedure void$java.lang.Object$$la$init$ra$$38($this:ref) returns ($exception:ref);    
+
+implementation void$NullPointerExceptions$add$1889($this:ref) returns ($exception:ref){
+    
+var $ex_return : bool;    
+var this1 : ref;
+    assume $this != $null;
+    $ex_return := false;
+    this1 := $this;
+    return;
+}
 
 
+implementation void$NullPointerExceptions$test$1890($this:ref) returns ($exception:ref){
+    
+var $fakelocal_0 : ref;    
+var obj14 : ref;    
+var $ex_return : bool;    
+var choice3 : int;    
+var this2 : ref;    
+var temp$05 : ref;
+    assume $this != $null;
+    $ex_return := false;
+    this2 := $this;
+    choice3 := 1;
+    obj14 := $null;
+    if (choice3 == 1) {
+        goto block1;
+    }
+    goto block2;
+  block1:
+    temp$05 := $null;
+    obj14 := temp$05;
+    if (obj14 != $null) {
+        $exception := $exception;
+    } else {
+        havoc $fakelocal_0;
+        assume !$heap[$fakelocal_0,$alloc];
+        $heap := $heap[$fakelocal_0,$alloc := true];
+        assume $fakelocal_0 != $null;
+        $heap := $heap[$fakelocal_0,$type := java.lang.NullPointerException];
+        $exception := $fakelocal_0;
+        $ex_return := true;
+        return;
+    }
+    if ($heap[obj14,$type] <: NullPointerExceptions && NullPointerExceptions <: $heap[obj14,$type]) {
+        call $exception := void$NullPointerExceptions$add$1889(obj14);
+    }
+  block2:
+    return;
+    return;
+}
 
 
-
-
-
-
-
-
-
-
-
-
-
-
-
+implementation void$NullPointerExceptions$$la$init$ra$$1891($this:ref) returns ($exception:ref){
+    
+var this6 : ref;    
+var $ex_return : bool;
+    assume $this != $null;
+    $ex_return := false;
+    this6 := $this;
+    call $exception := void$java.lang.Object$$la$init$ra$$38(this6);
+    return;
+}
 
 
